proofs

Semantics.thy
@@ -32,6 +32,7 @@ definition is_nbd_struct :: "'a Nbd_Struct \<Rightarrow> bool" where
   \<and> (\<forall>g. ( (GameInterp S g) \<in> carrier_of (World S) ))
   \<and> (\<forall>p. (PropInterp S p) \<subseteq> (World S)) "
 
+
 \<comment>\<open>valuation\<close>
 type_synonym 'a val = "var_type \<Rightarrow> 'a eff_fn_type"
 
@@ -48,13 +49,22 @@ definition ALL_CX :: "(Atm_game \<Rightarrow> int) set" where
 "ALL_CX = \<int> \<rightarrow> Sab"
 
 definition is_cx :: "cx \<Rightarrow> bool" where
-  "is_cx C \<equiv> \<forall>g::Atm_game. C g\<in>Sab"
+  "is_cx c \<equiv> c \<in> ALL_CX"
 
 definition dual_cx :: "cx \<Rightarrow> cx" where
   "dual_cx cx = -cx"
 
-fun subst_cx :: "cx \<Rightarrow> Atm_game \<Rightarrow> int \<Rightarrow> cx" where
+definition subst_cx :: "cx \<Rightarrow> Atm_game \<Rightarrow> int \<Rightarrow> cx" where
   "subst_cx f a i b = (if a=b then i else f b)"
+
+lemma subst_cx_compat :
+  assumes "c\<in> ALL_CX"
+  shows "subst_cx c a 1 \<in> ALL_CX \<and> subst_cx c a (-1)\<in> ALL_CX"
+  apply (auto simp add:Sab_def ALL_CX_def subst_cx_def)
+proof -
+  show "\<And>x. x \<in> \<int> \<Longrightarrow> c x \<noteq> - 1 \<Longrightarrow> c x \<noteq> 0 \<Longrightarrow> a \<noteq> x \<Longrightarrow> c x = 1" using assms by (auto simp add:ALL_CX_def Sab_def)
+  show "\<And>x. x \<in> \<int> \<Longrightarrow> c x \<noteq> - 1 \<Longrightarrow> c x \<noteq> 0 \<Longrightarrow> a \<noteq> x \<Longrightarrow> c x = 1" using assms by (auto simp add:ALL_CX_def Sab_def)
+qed
 
 definition dual_eff_fn :: "'a Nbd_Struct  \<Rightarrow> 'a eff_fn_type \<Rightarrow> 'a eff_fn_type" where
   "dual_eff_fn N f A = World N - ( f ( World N - A ) )"
@@ -74,11 +84,11 @@ definition sabo_dual :: "GLs_ground_type Nbd_Struct \<Rightarrow> GLs_eff_fn_typ
   "sabo_dual N f A = sabo_comp N (f (sabo_comp N A))"
 
 \<comment>\<open>function that substitutes atomic game "a" to Angelic control in context\<close>
-definition GLs_game_subst :: "GLs_sub_world_type \<Rightarrow> Atm_game \<Rightarrow> GLs_sub_world_type" where
-  "GLs_game_subst A a = {(w,c). (w,(subst_cx c a 1)) \<in> A}"
+definition GLs_game_subst :: "GLs_ground_type Nbd_Struct \<Rightarrow> GLs_sub_world_type \<Rightarrow> Atm_game \<Rightarrow> GLs_sub_world_type" where
+  "GLs_game_subst N A a = {(w,c)\<in> World N. (w,(subst_cx c a 1)) \<in> A}"
 
-definition GLs_game_Dsubst :: "GLs_sub_world_type \<Rightarrow> Atm_game \<Rightarrow> GLs_sub_world_type" where
-  "GLs_game_Dsubst A a = {(w,c). (w,(subst_cx c a (-1))) \<in> A}"
+definition GLs_game_Dsubst :: "GLs_ground_type Nbd_Struct \<Rightarrow> GLs_sub_world_type \<Rightarrow> Atm_game \<Rightarrow> GLs_sub_world_type" where
+  "GLs_game_Dsubst N A a = {(w,c) \<in> World N. (w,(subst_cx c a (-1))) \<in> A}"
 
 definition GLs_dual_eff_fn :: "GLs_ground_type Nbd_Struct \<Rightarrow> GLs_eff_fn_type \<Rightarrow> GLs_eff_fn_type" where
 "GLs_dual_eff_fn N f A = sabo_comp N (f (sabo_comp N A))"
@@ -116,14 +126,37 @@ definition lift_game_interp :: "ground_type Nbd_Struct \<Rightarrow> (Atm_game \
 "lift_game_interp N a (U:: (int\<times>(int \<Rightarrow> int)) set)
   ={(w,c). (c a = 0) \<and> (w \<in> (GameInterp N) a (fst ` U)) \<or> (c a = 1) \<and> ((w,c)\<in> U)}"
 
-fun lift_prop_interp :: "ground_type Nbd_Struct \<Rightarrow> Atm_fml \<Rightarrow> GLs_ground_type sub_world_type" where
+definition lift_prop_interp :: "ground_type Nbd_Struct \<Rightarrow> Atm_fml \<Rightarrow> GLs_ground_type sub_world_type" where
 "lift_prop_interp N P = (PropInterp N P) \<times> ALL_CX"
 
-fun GLs_lift_nbd :: "ground_type Nbd_Struct \<Rightarrow> GLs_ground_type Nbd_Struct" where
+definition GLs_lift_nbd :: "ground_type Nbd_Struct \<Rightarrow> GLs_ground_type Nbd_Struct" where
   "GLs_lift_nbd N = \<lparr> World=(World N)\<times>ALL_CX , 
     PropInterp = lift_prop_interp N,
     GameInterp = lift_game_interp N 
  \<rparr>"
+
+lemma sab_negate_compat : "a\<in>Sab \<Longrightarrow> -a\<in>Sab" by (auto simp add:Sab_def)
+
+lemma cx_negate_compat : 
+  assumes "b\<in>ALL_CX"
+  shows"-b\<in> ALL_CX"
+  using assms by (auto simp add:ALL_CX_def Sab_def)
+
+
+\<comment>\<open> Complement takes negative \<close>
+lemma sabo_dbl_comp : 
+  assumes "A \<subseteq> World N \<times> ALL_CX"
+  shows "sabo_comp (GLs_lift_nbd N) (sabo_comp (GLs_lift_nbd N) A) = A"
+  apply (auto simp add:sabo_comp_def dual_cx_def GLs_lift_nbd_def)
+proof -
+  show "\<And>a b. a \<in> World N \<Longrightarrow> b \<in> ALL_CX \<Longrightarrow> - b \<notin> ALL_CX \<Longrightarrow> (a, b) \<in> A" by (simp add: cx_negate_compat)
+  show "\<And>a b. a \<in> World N \<Longrightarrow> b \<in> ALL_CX \<Longrightarrow> (a, - (- b)) \<in> A \<Longrightarrow> (a, b) \<in> A"
+    using uminus_apply by fastforce
+  show "\<And>a b. (a, b) \<in> A \<Longrightarrow> a \<in> World N" using assms by auto
+  show "\<And>a b. (a, b) \<in> A \<Longrightarrow> b \<in> ALL_CX" using assms by auto
+  show "\<And>a b. (a, b) \<in> A \<Longrightarrow> - b \<in> ALL_CX \<Longrightarrow> a \<in> World N \<Longrightarrow> (a, - (- b)) \<in> A"
+    by (simp add: fun_Compl_def)
+qed
 
 fun GLs_fml_sem :: "GLs_ground_type Nbd_Struct \<Rightarrow> GLs_fml \<Rightarrow> GLs_sub_world_type"
  and GLs_game_sem :: "GLs_ground_type Nbd_Struct => GLs_game => GLs_eff_fn_type"
@@ -134,7 +167,7 @@ fun GLs_fml_sem :: "GLs_ground_type Nbd_Struct \<Rightarrow> GLs_fml \<Rightarro
 | "GLs_fml_sem N (GLs_Mod g f) = (GLs_game_sem N g) (GLs_fml_sem N f)"
 | "GLs_game_sem N (GLs_Atm_Game i) A = GameInterp N i A"
 | "GLs_game_sem N (GLs_Test fml) A = (GLs_fml_sem N fml) \<inter> A "
-| "GLs_game_sem N (GLs_Sabo a) A = GLs_game_subst A a"
+| "GLs_game_sem N (GLs_Sabo a) A = GLs_game_subst N A a"
 | "GLs_game_sem N (GLs_Dual g) A = sabo_dual N (GLs_game_sem N g) A"
 | "GLs_game_sem N (GLs_Choice a b) A = (GLs_game_sem N a A) \<union> (GLs_game_sem N b A)"
 | "GLs_game_sem N (GLs_Seq a b) A = GLs_game_sem N a (GLs_game_sem N b A)"
@@ -150,8 +183,8 @@ fun GLs_ext_fml_sem :: "GLs_ground_type Nbd_Struct \<Rightarrow> GLs_ext_fml \<R
 | "GLs_ext_fml_sem N (GLs_ext_And f1 f2) = (GLs_ext_fml_sem N f1) \<inter> (GLs_ext_fml_sem N f2)"
 | "GLs_ext_fml_sem N (GLs_ext_Mod g f) = GLs_ext_game_sem N g (GLs_ext_fml_sem N f)"
 | "GLs_ext_game_sem N (GLs_ext_Atm_Game a) A = (GameInterp N) a A"
-| "GLs_ext_game_sem N (GLs_ext_Sabo a) A = GLs_game_subst A a"
-| "GLs_ext_game_sem N (GLs_ext_DSabo a) A = GLs_game_Dsubst A a"
+| "GLs_ext_game_sem N (GLs_ext_Sabo a) A = GLs_game_subst N A a"
+| "GLs_ext_game_sem N (GLs_ext_DSabo a) A = GLs_game_Dsubst N A a"
 | "GLs_ext_game_sem N (GLs_ext_Dual g) A = GLs_dual_eff_fn N (GLs_ext_game_sem N g) A"
 | "GLs_ext_game_sem N (GLs_ext_Test f) A = A \<inter> GLs_ext_fml_sem N f"
 | "GLs_ext_game_sem N (GLs_ext_DTest f) A = (sabo_comp N A) \<union> sabo_comp N (GLs_ext_fml_sem N f)"
@@ -161,22 +194,56 @@ fun GLs_ext_fml_sem :: "GLs_ground_type Nbd_Struct \<Rightarrow> GLs_ext_fml \<R
 | "GLs_ext_game_sem N (GLs_ext_Star g) A = \<Inter> { B \<in> Pow (World N). A \<union> GLs_ext_game_sem N g B \<subseteq> B}"
 | "GLs_ext_game_sem N (GLs_ext_Cross g) A = \<Union> { B \<in> Pow (World N). B \<subseteq> A \<union> GLs_ext_game_sem N g B}"
 
+lemma cx_double_neg : 
+  assumes "c \<in> ALL_CX" shows "subst_cx c x (-1) = - subst_cx (- c) x 1" by (auto simp add:subst_cx_def)
+
+lemma cx_neg_sub:
+  assumes "c\<in> ALL_CX" shows "- (subst_cx c x t) = subst_cx (-c) x (-t)" by (auto simp add:subst_cx_def)
+
 lemma GLs_syn_inversion_compat :
-  fixes N:: "GLs_ground_type Nbd_Struct"
+  fixes N:: "ground_type Nbd_Struct"
   and f:: "GLs_ext_fml"
   and g:: "GLs_ext_game"
-assumes isStruct: "is_Nbd_Struct N"
-shows "GLs_ext_fml_sem N (GLs_syn_comp f) = sabo_comp N (GLs_ext_fml_sem N f)"
-   "GLs_ext_game_sem N (GLs_syn_dual g) A = GLs_dual_eff_fn N (GLs_ext_game_sem N g) A"
+assumes isStruct: "is_nbd_struct N"
+  and isStructlift: "is_nbd_struct (GLs_lift_nbd N)"
+shows "GLs_ext_fml_sem (GLs_lift_nbd N) (GLs_syn_comp f) = sabo_comp (GLs_lift_nbd N) (GLs_ext_fml_sem (GLs_lift_nbd N) f)"
+   "GLs_ext_game_sem (GLs_lift_nbd N) (GLs_syn_dual g) = GLs_dual_eff_fn (GLs_lift_nbd N) (GLs_ext_game_sem (GLs_lift_nbd N) g)"
 proof (induction f and g)
   case (GLs_ext_Atm_Game x)
-  then show ?case by (auto simp add:GLs_dual_eff_fn_def)
+  then show ?case by (auto simp add: GLs_dual_eff_fn_def )
 next
   case (GLs_ext_Sabo x)
-  then show ?case by (simp add:GLs_dual_eff_fn_def)
+  then show ?case
+    apply (auto simp add: isStructlift
+       GLs_lift_nbd_def  GLs_dual_eff_fn_def sabo_comp_def dual_cx_def GLs_game_subst_def GLs_game_Dsubst_def)
+    apply (rule)
+  proof
+    fix xa show " {(w, c). w \<in> World N \<and> c \<in> ALL_CX \<and> (w, subst_cx c x (- 1)) \<in> xa}
+          \<subseteq> {(w, cx). w \<in> World N \<and> cx \<in> ALL_CX \<and> (subst_cx (- cx) x 1 \<in> ALL_CX \<longrightarrow> w \<in> World N \<longrightarrow> - cx \<in> ALL_CX \<longrightarrow> (w, - subst_cx (- cx) x 1) \<in> xa)}"
+      by (auto simp add:cx_double_neg)
+    fix xa show "{(w, cx). w \<in> World N \<and> cx \<in> ALL_CX \<and> (subst_cx (- cx) x 1 \<in> ALL_CX \<longrightarrow> w \<in> World N \<longrightarrow> - cx \<in> ALL_CX \<longrightarrow> (w, - subst_cx (- cx) x 1) \<in> xa)}
+          \<subseteq> {(w, c). w \<in> World N \<and> c \<in> ALL_CX \<and> (w, subst_cx c x (- 1)) \<in> xa}  "
+      by (auto simp add:cx_double_neg cx_negate_compat subst_cx_compat)
+  qed
 next
   case (GLs_ext_DSabo x)
-  then show ?case sorry
+  then show ?case
+    apply (auto simp add: isStructlift
+    GLs_lift_nbd_def  GLs_dual_eff_fn_def sabo_comp_def dual_cx_def GLs_game_subst_def GLs_game_Dsubst_def)
+    apply rule
+  proof - fix xa show "{(w, c). w \<in> World N \<and> c \<in> ALL_CX \<and> (w, subst_cx c x 1) \<in> xa} =
+          {(w, cx). w \<in> World N \<and> cx \<in> ALL_CX \<and> (subst_cx (- cx) x (- 1) \<in> ALL_CX \<longrightarrow> w \<in> World N \<longrightarrow> - cx \<in> ALL_CX \<longrightarrow> (w, - subst_cx (- cx) x (- 1)) \<in> xa)}"
+      apply (auto simp add: isStructlift ALL_CX_def
+    GLs_lift_nbd_def  GLs_dual_eff_fn_def sabo_comp_def dual_cx_def GLs_game_subst_def GLs_game_Dsubst_def)
+    proof (metis (lifting) ext ALL_CX_def cx_neg_sub uminus_apply verit_minus_simplify(4))
+      fix a b xb show " a \<in> World N \<Longrightarrow> b \<in> \<int> \<rightarrow> Sab \<Longrightarrow> xb \<in> \<int> \<Longrightarrow> subst_cx (- b) x (- 1) xb \<notin> Sab \<Longrightarrow> (a, subst_cx b x 1) \<in> xa"
+        by (metis ALL_CX_def Pi_mem cx_negate_compat subst_cx_compat)
+      fix a b xb show "a \<in> World N \<Longrightarrow> b \<in> \<int> \<rightarrow> Sab \<Longrightarrow> xb \<in> \<int> \<Longrightarrow> - b xb \<notin> Sab \<Longrightarrow> (a, subst_cx b x 1) \<in> xa"
+        by (metis Pi_mem sab_negate_compat)
+      fix a b show "a \<in> World N \<Longrightarrow> b \<in> \<int> \<rightarrow> Sab \<Longrightarrow> (a, - subst_cx (- b) x (- 1)) \<in> xa \<Longrightarrow> (a, subst_cx b x 1) \<in> xa"
+        by (metis (lifting) ext ALL_CX_def cx_neg_sub uminus_apply verit_minus_simplify(4))
+    qed
+  qed
 next
   case (GLs_ext_Dual x)
   then show ?case sorry
